Logic/Modal/Standard/Kripke/Semantics.lean
@@ -29,206 +29,249 @@ end RelItr
 namespace Kripke
 
 
-structure Frame (α : Type*) where
-  World : Type*
-  [World_nonempty : Nonempty World]
-  Rel : World → World → Prop
+structure Frame (α) where
+  World : Set α
+  World_nonempty : World.Nonempty := by aesop
+  Rel : Set (World × World)
 
 structure FiniteFrame (α) extends Frame α where
-  [World_finite : Finite World]
+  World_finite : World.Finite := by simp;
 
-instance (F : Frame α) : Nonempty F.World := F.World_nonempty
+instance (F : Frame α) : F.World.Nonempty := F.World_nonempty
 
+/-
 instance : CoeSort (Frame α) (Type*) := ⟨Frame.World⟩
 
 instance : CoeFun (Frame α) (λ F => F.World → F.World → Prop) := ⟨Frame.Rel⟩
+-/
 
 instance : Coe (FiniteFrame α) (Frame α) := ⟨λ F ↦ F.toFrame⟩
 
-abbrev Frame.Rel' {F : Frame α} (w w' : F.World) := F.Rel w w'
+abbrev Frame.Rel' {F : Frame α} (x y : F.World) := (x, y) ∈ F.Rel
 scoped infix:45 " ≺ " => Frame.Rel'
 
-protected abbrev Frame.RelItr' (n : ℕ) {F : Frame α} (w w' : F.World) : Prop := RelItr (· ≺ ·) n w w'
-scoped notation w:45 " ≺^[" n "] " w':46 => Frame.RelItr' n w w'
+protected abbrev Frame.RelItr'  {F : Frame α} (n : ℕ) (x y : F.World) : Prop := RelItr (· ≺ ·) n x y
+scoped notation x:45 " ≺^[" n "] " y:46 => Frame.RelItr' n x y
 
 
 protected def Frame.finite (F : Frame α) := Finite F.World
 
+/-- dependent-version frame -/
+abbrev Frame' (α) (β : Type*) := Frame α
+
 
 /-- Frame with single world and identiy relation -/
-abbrev TerminalFrame (α) : FiniteFrame α := { World := PUnit, Rel := (· = ·) }
+abbrev TerminalFrame : FiniteFrame (Fin 1) where
+  World := {0}
+  Rel := { (x, y) | x = y }
 
 @[simp]
-lemma TerminalFrame.iff_rel' : Frame.Rel' (F := (TerminalFrame α).toFrame) x y ↔ x = y := by aesop;
+lemma TerminalFrame.iff_rel' {x y : TerminalFrame.World} : x ≺ y ↔ x = y := by
+  simp [Frame.Rel'];
 
 @[simp]
-lemma TerminalFrame.iff_relItr' : Frame.RelItr' n (F := (TerminalFrame α).toFrame) x y ↔ x = y := by
-  induction n with
-  | zero => simp;
-  | succ n ih => simp_all; use x;
+lemma TerminalFrame.iff_relItr' {x y : TerminalFrame.World} : x ≺^[n] y ↔ x = y := by
+  induction n <;> simp_all [Frame.Rel'];
 
 
-abbrev PointFrame (α) : FiniteFrame α := { World := PUnit, Rel := (· ≠ ·) }
+abbrev PointFrame : FiniteFrame (Fin 1) where
+  World := {0}
+  Rel := ∅
 
 
+abbrev FrameClass := ∀ (α : Type*), Set (Frame α)
 
-abbrev FrameClass (α) := Set (Frame α)
+/-- dependent-version frame class -/
+abbrev FrameClass' (β : Type*) := FrameClass
+
+
+abbrev FrameClass.union (𝔽₁ 𝔽₂ : FrameClass) : FrameClass := λ α => 𝔽₁ α ∪ 𝔽₂ α
+instance : Union FrameClass := ⟨FrameClass.union⟩
+
+abbrev FrameClass.inter (𝔽₁ 𝔽₂ : FrameClass) : FrameClass := λ α => 𝔽₁ α ∩ 𝔽₂ α
+instance : Inter FrameClass := ⟨FrameClass.inter⟩
+
+abbrev FrameClass.Nonempty (𝔽 : FrameClass) := ∃ (α : Type), (𝔽 α).Nonempty
+
+abbrev FrameClass.UNonempty (𝔽 : FrameClass) := ∃ (α : Type*), (𝔽 α).Nonempty
+
+-- def FrameClass.mem (F : Frame α) (𝔽 : FrameClass) : Prop := F ∈ 𝔽 α
 
 abbrev FiniteFrameClass (α) := Set (FiniteFrame α)
 
-def FrameClass.toFinite (𝔽 : FrameClass α) : FrameClass α := { F ∈ 𝔽 | F.finite }
+/-
+def FrameClass.toFinite (𝔽 : FrameClass) : FrameClass := ∀ α, { F | F ∈ 𝔽 α }
 postfix:max "ᶠ" => FrameClass.toFinite
+-/
 
-abbrev Valuation (W : Type u) (α : Type u) := W → α → Prop
+abbrev Valuation (F : Frame α) (β : Type*) := (F.World) → β → Prop
 
-structure Model (α) where
+structure Model (α β) where
   Frame : Frame α
-  Valuation : Valuation Frame.World α
+  Valuation : Valuation Frame β
 
-abbrev Model.World (M : Model α) := M.Frame.World
-instance : CoeSort (Model α) (Type _) where coe := Model.World
+abbrev Model.World (M : Model α β) := M.Frame.World
+-- instance : CoeSort (Model α) (Type _) where coe := Model.World
 
 
 end Kripke
 
 
-variable {α : Type*}
+variable {α β : Type*}
 
 open Standard.Kripke
 
-def Formula.kripke_satisfies (M : Kripke.Model α) (w : M.World) : Formula α → Prop
-  | atom a  => M.Valuation w a
+def Formula.kripke_satisfies (M : Kripke.Model α β) (x : M.World) : Formula β → Prop
+  | atom a  => M.Valuation x a
   | verum   => True
   | falsum  => False
-  | and p q => (kripke_satisfies M w p) ∧ (kripke_satisfies M w q)
-  | or p q  => (kripke_satisfies M w p) ∨ (kripke_satisfies M w q)
-  | imp p q => (kripke_satisfies M w p) → (kripke_satisfies M w q)
-  | box p   => ∀ {x}, w ≺ x → (kripke_satisfies M x p)
+  | and p q => (kripke_satisfies M x p) ∧ (kripke_satisfies M x q)
+  | or p q  => (kripke_satisfies M x p) ∨ (kripke_satisfies M x q)
+  | imp p q => (kripke_satisfies M x p) → (kripke_satisfies M x q)
+  | box p   => ∀ {y}, x ≺ y → (kripke_satisfies M y p)
 
 namespace Formula.kripke_satisfies
 
-protected instance semantics (M : Model α) : Semantics (Formula α) (M.World) := ⟨fun w ↦ Formula.kripke_satisfies M w⟩
+protected instance semantics : Semantics (Formula β) ((M : Model α β) × M.World) := ⟨fun ⟨M, x⟩ ↦ Formula.kripke_satisfies M x⟩
 
-variable {M : Model α} {w : M.World} {p q : Formula α}
+variable {M : Model α β} {x : ↑M.World} {p q : Formula β}
 
-@[simp] protected lemma iff_models : w ⊧ f ↔ kripke_satisfies M w f := iff_of_eq rfl
+notation:max "(" M ", " x ")" " ⊧ " p:50 => Formula.kripke_satisfies M x p
 
-lemma dia_def  : w ⊧ ◇p ↔ ∃ w', w ≺ w' ∧ w' ⊧ p := by simp [kripke_satisfies];
+@[simp] protected lemma iff_models : (⟨M, x⟩ : (M : Model α β) × ↑M.World) ⊧ p ↔ kripke_satisfies M x p := iff_of_eq rfl
 
-lemma multibox_def : w ⊧ □^[n]p ↔ ∀ v, w ≺^[n] v → v ⊧ p := by
-  induction n generalizing w with
-  | zero => simp;
+
+protected instance tarski : Semantics.Tarski ((M : Model α β) × M.World) where
+  realize_top := by intro; trivial;
+  realize_bot := by aesop;
+  realize_not := by aesop;
+  realize_and := by
+    intro ⟨M, x⟩ p q;
+    constructor;
+    . intro ⟨hp, hq⟩; exact ⟨hp, hq⟩;
+    . intro h; exact ⟨h.1, h.2⟩;
+  realize_or  := by aesop;
+  realize_imp := by aesop;
+
+
+lemma dia_def : (M, x) ⊧ ◇p ↔ ∃ (y : M.World), x ≺ y ∧ (M, y) ⊧ p := by simp [kripke_satisfies];
+
+lemma multibox_def : (M, x) ⊧ □^[n]p ↔ ∀ {y : M.World}, x ≺^[n] y → (M, y) ⊧ p := by
+  induction n generalizing x with
+  | zero => aesop;
   | succ n ih =>
     constructor;
-    . intro h w' hww';
-      simp at h;
-      obtain ⟨v, hwv, hvw'⟩ := hww';
-      exact (ih.mp $ h hwv) w' hvw';
+    . intro h y Rxy;
+      simp [kripke_satisfies] at h;
+      obtain ⟨u, hxu, huy⟩ := Rxy;
+      exact (ih.mp $ h u (by simp_all) hxu) huy;
     . simp;
-      intro h w' hww';
+      intro h y Rxy;
       apply ih.mpr;
-      intro v hwv;
-      exact h v w' hww' hwv;
+      intro u Ryu;
+      exact h u u.2 y y.2 Rxy Ryu;
 
-lemma multidia_def : w ⊧ ◇^[n]p ↔ ∃ v, w ≺^[n] v ∧ v ⊧ p := by
-  induction n generalizing w with
+lemma multidia_def : (M, x) ⊧ ◇^[n]p ↔ ∃ y, x ≺^[n] y ∧ (M, y) ⊧ p := by
+  induction n generalizing x with
   | zero => simp;
   | succ n ih =>
     constructor;
     . intro h;
-      replace h : kripke_satisfies M w (◇◇^[n]p) := by simpa using h;
+      replace h : (M, x) ⊧ (◇◇^[n]p) := by simpa using h;
       obtain ⟨v, hwv, hv⟩ := dia_def.mp h;
       obtain ⟨x, hvx, hx⟩ := ih.mp hv;
       use x;
       constructor;
       . use v;
       . assumption;
-    . simp [dia_def];
-      intro x y hwy hyx hx;
-      simp [kripke_satisfies];
-      use y;
+    . intro h;
+      obtain ⟨y, Rxy, hy⟩ := h;
+      obtain ⟨u, Rxu, Ruy⟩ := Rxy;
+      simp;
+      apply dia_def.mpr;
+      use u;
       constructor;
-      . assumption;
+      . exact Rxu;
       . apply ih.mpr;
-        existsi x;
-        simp_all;
-
-instance : Semantics.Tarski M.World where
-  realize_top := by simp [kripke_satisfies];
-  realize_bot := by simp [kripke_satisfies];
-  realize_not := by simp [kripke_satisfies];
-  realize_and := by simp [kripke_satisfies];
-  realize_or  := by simp [kripke_satisfies];
-  realize_imp := by simp [kripke_satisfies];
+        use y;
 
 end Formula.kripke_satisfies
 
 
-def Formula.valid_on_KripkeModel (M : Model α) (f : Formula α) := ∀ w : M.World, w ⊧ f
+def Formula.valid_on_KripkeModel (M : Model α β) (f : Formula β) := ∀ w, (M, w) ⊧ f
 
 namespace Formula.valid_on_KripkeModel
 
-protected instance : Semantics (Formula α) (Model α) := ⟨fun M ↦ Formula.valid_on_KripkeModel M⟩
+protected instance : Semantics (Formula β) (Model α β) := ⟨fun M ↦ Formula.valid_on_KripkeModel M⟩
 
-@[simp] protected lemma iff_models {M : Model α} : M ⊧ f ↔ valid_on_KripkeModel M f := iff_of_eq rfl
+@[simp] protected lemma iff_models {M : Model α β} : M ⊧ f ↔ valid_on_KripkeModel M f := iff_of_eq rfl
 
-instance : Semantics.Bot (Model α) where
-  realize_bot _ := by simp [valid_on_KripkeModel];
+instance : Semantics.Bot (Model α β) where
+  realize_bot M := by
+    obtain ⟨x, hx⟩ := M.Frame.World_nonempty;
+    simp [valid_on_KripkeModel, kripke_satisfies];
+    use x, hx;
+
 
 end Formula.valid_on_KripkeModel
 
 
-def Formula.valid_on_KripkeFrame (F : Frame α) (f : Formula α) := ∀ V, (Model.mk F V) ⊧ f
+def Formula.valid_on_KripkeFrame (F : Frame α) (p : Formula β) := ∀ V : Valuation F β, (⟨F, V⟩ : Model α β) ⊧ p
 
 namespace Formula.valid_on_KripkeFrame
 
-protected instance semantics : Semantics (Formula α) (Frame α) := ⟨fun F ↦ Formula.valid_on_KripkeFrame F⟩
+protected instance semantics : Semantics (Formula β) (Frame' α β) := ⟨fun F ↦ Formula.valid_on_KripkeFrame F⟩
 
-@[simp] protected lemma models_iff {F : Frame α} : F ⊧ f ↔ valid_on_KripkeFrame F f := iff_of_eq rfl
+variable {F : Frame' α β}
 
-instance : Semantics.Bot (Frame α) where
+@[simp] protected lemma models_iff : F ⊧ p ↔ valid_on_KripkeFrame F p := iff_of_eq rfl
+
+
+instance : Semantics.Bot (Frame' α β) where
   realize_bot _ := by simp [valid_on_KripkeFrame];
 
-protected lemma axiomK {F : Frame α} : F ⊧* 𝗞 := by
-  simp [valid_on_KripkeFrame, valid_on_KripkeModel, System.Axioms.K];
-  intro f p q ef V x; subst ef;
-  intro h₁ h₂ y rxy;
-  exact h₁ rxy (h₂ rxy);
 
-protected lemma nec {F : Frame α} (h : F ⊧ p) : F ⊧ □p := by
+protected lemma axiomK : F ⊧* 𝗞 := by
+  simp [valid_on_KripkeFrame, valid_on_KripkeModel, System.Axioms.K];
+  intro _ p q epq V x hx; subst epq;
+  intro h₁ h₂ y rxy;
+  exact h₁ rxy $ h₂ rxy;
+
+protected lemma nec (h : F ⊧ p) : F ⊧ □p := by
   intro V x y _;
   exact h V y;
 
-protected lemma mdp {F : Frame α} (hpq : F ⊧ p ⟶ q) (hp : F ⊧ p) : F ⊧ q := by
+protected lemma mdp (hpq : F ⊧ p ⟶ q) (hp : F ⊧ p) : F ⊧ q := by
   intro V x;
   exact (hpq V x) (hp V x);
 
 end Formula.valid_on_KripkeFrame
 
 
-@[simp] def Formula.valid_on_KripkeFrameClass (𝔽 : FrameClass α) (p : Formula α) := ∀ F ∈ 𝔽, F ⊧ p
+@[simp] def Formula.valid_on_KripkeFrameClass (𝔽 : FrameClass) (p : Formula β) := ∀ {α}, ∀ (F : Frame' α β), F ∈ (𝔽 α) → F ⊧ p
 
 namespace Formula.valid_on_KripkeFrameClass
 
-protected instance semantics : Semantics (Formula α) (FrameClass α) := ⟨fun 𝔽 ↦ Formula.valid_on_KripkeFrameClass 𝔽⟩
+protected instance semantics : Semantics (Formula β) (FrameClass' β) := ⟨fun 𝔽 ↦ Formula.valid_on_KripkeFrameClass 𝔽⟩
 
-variable {𝔽 : FrameClass α}
+variable {𝔽 : FrameClass' β}
 
 @[simp] protected lemma models_iff : 𝔽 ⊧ f ↔ Formula.valid_on_KripkeFrameClass 𝔽 f := iff_of_eq rfl
 
+
 protected lemma axiomK : 𝔽 ⊧* 𝗞 := by
   simp only [Semantics.RealizeSet.setOf_iff];
-  rintro f ⟨p, q, _⟩ F _;
+  rintro f ⟨p, q, _⟩ _ F _;
   apply (Semantics.RealizeSet.setOf_iff.mp $ valid_on_KripkeFrame.axiomK) f;
   use p, q;
 
 protected lemma nec (h : 𝔽 ⊧ p) : 𝔽 ⊧ □p := by
-  intro F hF;
+  intro _ F hF;
   apply valid_on_KripkeFrame.nec;
   exact h F hF;
 
 protected lemma mdp (hpq : 𝔽 ⊧ p ⟶ q) (hp : 𝔽 ⊧ p) : 𝔽 ⊧ q := by
-  intro F hF;
+  intro _ F hF;
   exact valid_on_KripkeFrame.mdp (hpq F hF) (hp F hF)
 
 end Formula.valid_on_KripkeFrameClass
@@ -236,13 +279,13 @@ end Formula.valid_on_KripkeFrameClass
 
 namespace AxiomSet
 
-variable {Ax Ax₁ Ax₂ : AxiomSet α}
+variable {Ax Ax₁ Ax₂ : AxiomSet β}
 
-def DefinesKripkeFrameClass (Ax : AxiomSet α) (𝔽 : FrameClass α) := ∀ {F}, F ⊧* Ax ↔ F ∈ 𝔽
+def DefinesKripkeFrameClass (Ax : AxiomSet β) (𝔽 : FrameClass) := ∀ {α}, ∀ {F : Frame' α β}, F ⊧* Ax ↔ F ∈ (𝔽 α)
 
 lemma DefinesKripkeFrameClass.union (defines₁ : Ax₁.DefinesKripkeFrameClass 𝔽₁) (defines₂ : Ax₂.DefinesKripkeFrameClass 𝔽₂)
   : (Ax₁ ∪ Ax₂).DefinesKripkeFrameClass (𝔽₁ ∩ 𝔽₂) := by
-  intro F;
+  intro _ F;
   simp only [Semantics.RealizeSet.union_iff];
   constructor;
   . intro ⟨h₁, h₂⟩;
@@ -255,8 +298,9 @@ lemma DefinesKripkeFrameClass.union (defines₁ : Ax₁.DefinesKripkeFrameClass 
     . apply defines₂.mpr h₂;
 
 
-def FinitelyDefinesKripkeFrameClass (Ax : AxiomSet α) (𝔽 : FrameClass α) := ∀ {F}, F.finite → (F ⊧* Ax ↔ F ∈ 𝔽)
+def FinitelyDefinesKripkeFrameClass (Ax : AxiomSet β) (𝔽 : FrameClass' β) := ∀ {F : Frame' α β}, F.finite → (F ⊧* Ax ↔ F ∈ (𝔽 α))
 
+/-
 def FinitelyDefinesKripkeFrameClass.union (defines₁ : Ax₁.FinitelyDefinesKripkeFrameClass 𝔽₁) (defines₂ : Ax₂.FinitelyDefinesKripkeFrameClass 𝔽₂)
   : (Ax₁ ∪ Ax₂).FinitelyDefinesKripkeFrameClass (𝔽₁ ∩ 𝔽₂) := by
   intro F hF;
@@ -285,6 +329,7 @@ instance {𝔽 : FrameClass α} (ne : 𝔽ᶠ.Nonempty) : 𝔽.Nonempty := by
   simp [FrameClass.toFinite] at hF;
   use F;
   exact hF.1;
+-/
 
 end AxiomSet
 
@@ -294,19 +339,21 @@ namespace Kripke
 open Formula
 open AxiomSet (DefinesKripkeFrameClass)
 
-abbrev AllFrameClass (α) : FrameClass α := Set.univ
+abbrev AllFrameClass : FrameClass := λ _ => Set.univ
+abbrev AllFrameClass' (β : Type*) : FrameClass' β := AllFrameClass
 
-lemma AllFrameClass.nonempty : (AllFrameClass α).Nonempty := by
-  use TerminalFrame α; trivial;
+lemma AllFrameClass.nonempty : AllFrameClass.Nonempty := by
+  use Fin 1, TerminalFrame;
+  trivial;
 
-lemma axiomK_defines : 𝗞.DefinesKripkeFrameClass (AllFrameClass α) := by
+lemma axiomK_defines : 𝗞.DefinesKripkeFrameClass (β := β) (AllFrameClass) := by
   intro F;
   simp only [Set.mem_univ, iff_true];
   exact valid_on_KripkeFrame.axiomK;
 
-lemma axiomK_union_definability {Ax : AxiomSet α} {𝔽 : FrameClass α} : (Ax.DefinesKripkeFrameClass 𝔽) ↔ (𝗞 ∪ Ax).DefinesKripkeFrameClass 𝔽 := by
+lemma axiomK_union_definability {Ax : AxiomSet β} {𝔽 : FrameClass' β} : (Ax.DefinesKripkeFrameClass 𝔽) ↔ (𝗞 ∪ Ax).DefinesKripkeFrameClass 𝔽 := by
   constructor;
-  . intro defines F;
+  . intro defines _ F;
     simp [DefinesKripkeFrameClass] at defines;
     constructor;
     . intro h;
@@ -317,7 +364,7 @@ lemma axiomK_union_definability {Ax : AxiomSet α} {𝔽 : FrameClass α} : (Ax.
       constructor;
       . apply valid_on_KripkeFrame.axiomK;
       . exact defines.mpr h;
-  . intro defines F;
+  . intro defines _ F;
     simp only [DefinesKripkeFrameClass] at defines;
     constructor;
     . intro h;
@@ -331,12 +378,14 @@ lemma axiomK_union_definability {Ax : AxiomSet α} {𝔽 : FrameClass α} : (Ax.
       exact defines.mpr h |>.2;
 
 
+/-
 def nonempty_of_exist_finiteFrame {𝔽 : FrameClass α} (h : ∃ (F : FiniteFrame α), F.toFrame ∈ 𝔽) : 𝔽ᶠ.Nonempty := by
   obtain ⟨F, hF⟩ := h;
   use F.toFrame;
   constructor;
   . assumption;
   . exact F.World_finite;
+-/
 
 end Kripke
 
@@ -347,7 +396,7 @@ open Kripke
 variable {Λ Λ₁ Λ₂ : DeductionParameter α} [Λ.IsNormal]
 variable {Ax : AxiomSet α}
 
-abbrev DefinesKripkeFrameClass (Λ : DeductionParameter α) [Λ.IsNormal] (𝔽 : FrameClass α) := AxiomSet.DefinesKripkeFrameClass (Ax(Λ)) 𝔽
+abbrev DefinesKripkeFrameClass (Λ : DeductionParameter α) [Λ.IsNormal] (𝔽 : FrameClass) := AxiomSet.DefinesKripkeFrameClass (Ax(Λ)) 𝔽
 
 lemma DefinesKripkeFrameClass.toAx (defines : Λ.DefinesKripkeFrameClass 𝔽) : Ax(Λ).DefinesKripkeFrameClass 𝔽 := by
   simp [DefinesKripkeFrameClass] at defines;
@@ -362,7 +411,7 @@ lemma DefinesKripkeFrameClass.ofAx (defines : Ax.DefinesKripkeFrameClass 𝔽) [
   assumption;
 
 
-abbrev FinitelyDefinesKripkeFrameClass (Λ : DeductionParameter α) [Λ.IsNormal] (𝔽 : FrameClass α) := AxiomSet.FinitelyDefinesKripkeFrameClass (Ax(Λ)) 𝔽
+-- abbrev FinitelyDefinesKripkeFrameClass (Λ : DeductionParameter α) [Λ.IsNormal] (𝔽 : FrameClass) := AxiomSet.FinitelyDefinesKripkeFrameClass (Ax(Λ)) 𝔽
 
 end DeductionParameter
 
