Logic/Modal/Standard/Kripke/Preservation.lean
@@ -1,0 +1,83 @@
+import Logic.Modal.Standard.Kripke.Semantics
+
+namespace LO.Modal.Standard
+
+namespace Kripke
+
+
+section Bisimulation
+
+
+end Bisimulation
+
+
+section Generation
+
+class GeneratedSubframe (F F' : Kripke.Frame α) where
+  subset : F'.World ⊆ F.World
+  -- rel : ∀ x y : F'.World, F'.Rel' x y → F.Rel' x y
+  closed : ∀ x y : F.World, x ≺ y → y.1 ∈ F'.World
+
+
+end Generation
+
+
+section Reduction
+
+protected class Frame.reduction {F₁ F₂ : Kripke.Frame α} (f : F₁.World → F₂.World)  where
+  forth : ∀ {w v : F₁.World}, w ≺ v → (f w) ≺ (f v)
+  back : ∀ {w : F₁.World}, ∀ {v : F₂.World}, (f w) ≺ v → ∃ u, w ≺ u ∧ f u = v
+
+
+protected class Model.reduction {M₁ M₂ : Kripke.Model α β} (f : M₁.World → M₂.World)  extends Frame.reduction f where
+  atomic : ∀ {w : M₁.World}, ∀ {a}, (M₁.Valuation w a) ↔ (M₂.Valuation (f w) a)
+
+
+open Formula
+
+variable {F₁ F₂ : Kripke.Frame α} {M₁ M₂ : Kripke.Model α β}
+
+lemma iff_formula_satisfies_morphism (f : M₁.World → M₂.World) [Model.reduction f] {w : M₁.World} : (M₁, w) ⊧ p ↔ (M₂, (f w)) ⊧ p := by
+  induction p using Formula.rec' generalizing w with
+  | hatom p =>
+    constructor;
+    . apply Model.reduction.atomic |>.mp;
+    . apply Model.reduction.atomic |>.mpr
+  | hbox p ih =>
+    constructor;
+    . intro h w₂ hw₂;
+      obtain ⟨w₁, ⟨hww₁, e⟩⟩ := Frame.reduction.back hw₂;
+      have := ih.mp $ h hww₁;
+      subst e;
+      assumption;
+    . intro h w' hww';
+      exact ih.mpr $ h $ Frame.reduction.forth hww';
+  | _ => simp_all;
+
+lemma iff_formula_valid_on_frame_surjective_morphism (f : F₁ → F₂) [Frame.reduction f] (f_surjective : f.Surjective) : F₁ ⊧ p → F₂ ⊧ p := by
+  contrapose;
+  intro h;
+  obtain ⟨V₂, w₂, h⟩ := by simpa [valid_on_KripkeFrame, valid_on_KripkeModel] using h;
+  simp [valid_on_KripkeFrame, valid_on_KripkeModel];
+
+  obtain ⟨w₁, e⟩ : ∃ w₁, f w₁ = w₂ := by apply f_surjective;
+  subst e;
+  let V₁ := λ w a => V₂ (f w) a;
+  use V₁, w₁;
+
+  let M₁ : Model α := { Frame := F₁, Valuation := V₁ };
+  let M₂ : Model α := { Frame := F₂, Valuation := V₂ };
+  have : Model.reduction (M₁ := M₁) (M₂ := M₂) f := { atomic := by simp_all };
+  exact iff_formula_satisfies_morphism (M₁ := M₁) (M₂ := M₂) f |>.not.mpr h;
+
+lemma iff_theory_valid_on_frame_surjective_morphism (f : F₁ → F₂) [Frame.reduction f] (f_surjective : f.Surjective) : F₁ ⊧* T → F₂ ⊧* T := by
+  simp only [Semantics.realizeSet_iff];
+  intro h p hp;
+  exact iff_formula_valid_on_frame_surjective_morphism f f_surjective (h hp);
+
+end Reduction
+
+
+end Kripke
+
+end LO.Modal.Standard
